wip

src/SimulationRelAux.v
@@ -77,63 +77,6 @@ Proof.
   done.
 Qed.
 
-Definition closedness_preserved memory memory' :=
-  forall view,
-    Memory.closed_timemap view memory ->
-    Memory.closed_timemap view memory'.
-
-Lemma closedness_preserved_id memory :
-  closedness_preserved memory memory.
-Proof. by intros view. Qed.
-
-Lemma closedness_preserved_add memory memory'
-      loc from to val rel
-      (ADD : Memory.add memory loc from to val rel memory'):
-  closedness_preserved memory memory'.
-Proof.
-  intros view CP. red.
-  intros loc'.
-  erewrite Memory.add_o; eauto.
-  destruct (loc_ts_eq_dec (loc', view loc') (loc, to)) as [[A B]|NEQ]; simpls.
-  subst; eexists; eexists; eexists; eauto.
-Qed.
-
-Lemma closedness_preserved_split memory memory'
-      loc from to to' val val' rel rel'
-      (SPLIT : Memory.split memory loc from to to' val val' rel rel' memory'):
-  closedness_preserved memory memory'.
-Proof.
-  intros view CP. red.
-  intros loc'.
-  erewrite Memory.split_o; eauto.
-  destruct (loc_ts_eq_dec (loc', view loc') (loc, to)) as [[A B]|NEQ]; simpls.
-  { eexists; eexists; eexists; eauto. }
-  destruct (loc_ts_eq_dec (loc', view loc') (loc, to')) as [[A B]|NEQ']; simpls.
-  eexists; eexists; eexists; eauto.
-Qed.
-
-Lemma tview_closedness_preserved_add tview memory memory'
-      loc from to val rel
-      (ADD : Memory.add memory loc from to val rel memory')
-      (MEM_CLOSE : memory_close tview memory) :
-  memory_close tview memory'.
-Proof.
-  red; splits; ins.
-  all: eapply closedness_preserved_add; eauto.
-  all: by apply MEM_CLOSE.
-Qed.
-
-Lemma tview_closedness_preserved_split tview memory memory'
-      loc from to to' val val' rel rel'
-      (SPLIT : Memory.split memory loc from to to' val val' rel rel' memory')
-      (MEM_CLOSE : memory_close tview memory) :
-  memory_close tview memory'.
-Proof.
-  red; splits; ins.
-  all: eapply closedness_preserved_split; eauto.
-  all: by apply MEM_CLOSE.
-Qed.
-
 Lemma sim_msg_f_issued f_to f_to' T rel b 
       (TCCOH : tc_coherent G sc T)
       (IMMCON : imm_consistent G sc)
