src/lib/MemoryClosedness.v
@@ -1,0 +1,62 @@
+Require Import Setoid PArith.
+From hahn Require Import Hahn.
+Require Import PromisingLib.
+From Promising2 Require Import TView View Time Event Cell Thread Memory Configuration.
+Require Import MemoryAux.
+
+Definition closedness_preserved memory memory' :=
+  forall view,
+    Memory.closed_timemap view memory ->
+    Memory.closed_timemap view memory'.
+
+Lemma closedness_preserved_id memory :
+  closedness_preserved memory memory.
+Proof. by intros view. Qed.
+
+Lemma closedness_preserved_add memory memory'
+      loc from to msg 
+      (ADD : Memory.add memory loc from to msg memory'):
+  closedness_preserved memory memory'.
+Proof.
+  intros view CP. red.
+  intros loc'.
+  erewrite Memory.add_o; eauto.
+  destruct (loc_ts_eq_dec (loc', view loc') (loc, to)) as [[A B]|NEQ]; simpls.
+  subst; eexists; eexists; eexists; eauto.
+Qed.
+
+Lemma closedness_preserved_split memory memory'
+      loc from to to' val val' rel rel'
+      (SPLIT : Memory.split memory loc from to to' val val' rel rel' memory'):
+  closedness_preserved memory memory'.
+Proof.
+  intros view CP. red.
+  intros loc'.
+  erewrite Memory.split_o; eauto.
+  destruct (loc_ts_eq_dec (loc', view loc') (loc, to)) as [[A B]|NEQ]; simpls.
+  { eexists; eexists; eexists; eauto. }
+  destruct (loc_ts_eq_dec (loc', view loc') (loc, to')) as [[A B]|NEQ']; simpls.
+  eexists; eexists; eexists; eauto.
+Qed.
+
+Lemma tview_closedness_preserved_add tview memory memory'
+      loc from to val rel
+      (ADD : Memory.add memory loc from to val rel memory')
+      (MEM_CLOSE : memory_close tview memory) :
+  memory_close tview memory'.
+Proof.
+  red; splits; ins.
+  all: eapply closedness_preserved_add; eauto.
+  all: by apply MEM_CLOSE.
+Qed.
+
+Lemma tview_closedness_preserved_split tview memory memory'
+      loc from to to' val val' rel rel'
+      (SPLIT : Memory.split memory loc from to to' val val' rel rel' memory')
+      (MEM_CLOSE : memory_close tview memory) :
+  memory_close tview memory'.
+Proof.
+  red; splits; ins.
+  all: eapply closedness_preserved_split; eauto.
+  all: by apply MEM_CLOSE.
+Qed.
